Fix is_even example

examples/tutorial/2-lift/birExamples2BinaryScript.sml
@@ -11,14 +11,14 @@ val bprog_is_even_odd_def = Define `
       bb_statements :=
         [];
       bb_last_statement := BStmt_CJmp (BExp_BinPred BIExp_Equal
-                                                      (BExp_Den (BVar "n" (BType_Imm Bit32)))
-                                                      (BExp_Const (Imm32 0w)))
+                                                      (BExp_Den (BVar "n" (BType_Imm Bit64)))
+                                                      (BExp_Const (Imm64 0w)))
                                       (BLE_Label (BL_Address (Imm32 0x200w)))
                                       (BLE_Label (BL_Address (Imm32 0x004w)))|>;
     <|bb_label := BL_Address (Imm32 0x004w);
       bb_statements :=
-        [BStmt_Assign (BVar "n" (BType_Imm Bit32))
-                      (BExp_BinExp BIExp_Minus (BExp_Den (BVar "n" (BType_Imm Bit32))) (BExp_Const (Imm32 1w)));
+        [BStmt_Assign (BVar "n" (BType_Imm Bit64))
+                      (BExp_BinExp BIExp_Minus (BExp_Den (BVar "n" (BType_Imm Bit64))) (BExp_Const (Imm64 1w)));
         ];
       bb_last_statement := BStmt_Jmp (BLE_Label (BL_Address (Imm32 0x100w)))|>;
 
@@ -28,14 +28,14 @@ val bprog_is_even_odd_def = Define `
       bb_statements :=
         [];
       bb_last_statement := BStmt_CJmp (BExp_BinPred BIExp_Equal
-                                                      (BExp_Den (BVar "n" (BType_Imm Bit32)))
-                                                      (BExp_Const (Imm32 0w)))
+                                                      (BExp_Den (BVar "n" (BType_Imm Bit64)))
+                                                      (BExp_Const (Imm64 0w)))
                                       (BLE_Label (BL_Address (Imm32 0x204w)))
                                       (BLE_Label (BL_Address (Imm32 0x104w)))|>;
     <|bb_label := BL_Address (Imm32 0x104w);
       bb_statements :=
-        [BStmt_Assign (BVar "n" (BType_Imm Bit32))
-                      (BExp_BinExp BIExp_Minus (BExp_Den (BVar "n" (BType_Imm Bit32))) (BExp_Const (Imm32 1w)));
+        [BStmt_Assign (BVar "n" (BType_Imm Bit64))
+                      (BExp_BinExp BIExp_Minus (BExp_Den (BVar "n" (BType_Imm Bit64))) (BExp_Const (Imm64 1w)));
         ];
       bb_last_statement := BStmt_Jmp (BLE_Label (BL_Address (Imm32 0x000w)))|>;
 
@@ -46,6 +46,9 @@ val bprog_is_even_odd_def = Define `
         [BStmt_Assign (BVar "r" (BType_Imm Bit1))
                       (BExp_Const (Imm1 1w))
         ];
+      bb_last_statement := BStmt_Jmp (BLE_Label (BL_Address (Imm32 0x210w)))|>;
+    <|bb_label := BL_Address (Imm32 0x210w);
+      bb_statements := [];
       bb_last_statement := BStmt_Halt (BExp_Const (Imm32 0x0w))|>;
 
 
@@ -55,6 +58,9 @@ val bprog_is_even_odd_def = Define `
         [BStmt_Assign (BVar "r" (BType_Imm Bit1))
                       (BExp_Const (Imm1 0w))
         ];
+      bb_last_statement := BStmt_Jmp (BLE_Label (BL_Address (Imm32 0x214w)))|>;
+    <|bb_label := BL_Address (Imm32 0x214w);
+      bb_statements := [];
       bb_last_statement := BStmt_Halt (BExp_Const (Imm32 0x0w))|>
 ]) : 'a bir_program_t
 `;
