examples/tutorial/5-wp/tutorialExtra2_wpScript.sml
@@ -37,13 +37,14 @@ val prog_tm = (lhs o concl) bprog_is_even_odd_def;
 Sections and hoare triples:
 *)
 
-val get_n = bden (bvar "n" ``(BType_Imm Bit32)``);
+val get_n  = bden (bvar "n" ``(BType_Imm Bit64)``);
 
-val get_v1 = bconst ``v1:word32``;
+val get_v1 = bconst ``v1:word64``;
+val get_v  = bconst ``v :word64``;
 
-val get_0  = bconst ``0w:word32``;
-val get_1  = bconst ``1w:word32``;
-val get_2  = bconst ``2w:word32``;
+val get_0  = bconst ``0w:word64``;
+val get_1  = bconst ``1w:word64``;
+val get_2  = bconst ``2w:word64``;
 
 (* =============================================================== *)
 
@@ -60,28 +61,14 @@ val bir_ieo_ev_post_no_def = Define `bir_ieo_ev_post_no v1 =
 ^(beq (bmod (get_v1, get_2), get_1))
 `;
 
-
-(* overall contract is_odd *)
-val bir_ieo_od_pre_def = Define `bir_ieo_od_pre v1 =
-^(beq (get_n, get_v1))
-`;
-
-val bir_ieo_od_post_yes_def = Define `bir_ieo_od_post_yes v1 =
-^(beq (bmod (get_v1, get_2), get_1))
-`;
-
-val bir_ieo_od_post_no_def = Define `bir_ieo_od_post_no v1 =
-^(beq (bmod (get_v1, get_2), get_0))
-`;
-
 (* =============================================================== *)
 
 val bir_ieo_invariant_def = Define `bir_ieo_invariant v1 =
 ^(beq (bmod (get_v1, get_2), bmod (get_n, get_2)))
 `;
 
-val bir_ieo_invariant_mid_def = Define `bir_ieo_invariant_mid v1 =
-^(beq (bmod (get_v1, get_2), bmod (bplus(get_n, get_1), get_2)))
+val bir_ieo_condition_def = Define `bir_ieo_condition =
+^(bgt(get_n, get_1))
 `;
 
 val bir_ieo_variant_def = Define `bir_ieo_variant =
@@ -90,36 +77,24 @@ val bir_ieo_variant_def = Define `bir_ieo_variant =
 
 (* =============================================================== *)
 
-(* section is_even_1 *)
-val bir_ieo_sec_iseven_1_pre_def = Define `bir_ieo_sec_iseven_1_pre v1 =
-bir_ieo_invariant v1
+(* section is_even loop pre *)
+val bir_ieo_sec_iseven_loop_pre_def = Define `bir_ieo_sec_iseven_loop_pre v1 v =
+(BExp_BinExp BIExp_And (bir_ieo_invariant v1)
+                  (BExp_BinExp BIExp_And bir_ieo_condition
+                     (BExp_BinPred BIExp_Equal bir_ieo_variant ^(get_v))))
 `;
 
-val bir_ieo_sec_iseven_1_post_def = Define `bir_ieo_sec_iseven_1_post v1 =
+(* section is_even exit pre *)
+val bir_ieo_sec_iseven_exit_pre_def = Define `bir_ieo_sec_iseven_exit_pre v1 =
+(BExp_BinExp BIExp_And (bir_ieo_invariant v1) (BExp_UnaryExp BIExp_Not bir_ieo_condition))
+`;
+
+
+(* section is_even post *)
+val bir_ieo_sec_iseven_post_def = Define `bir_ieo_sec_iseven_post v1 =
 \l. if l = BL_Address (Imm32 0x200w) then
       bir_ieo_ev_post_yes v1
-    else if l = BL_Address (Imm32 0x100w) then
-      bir_ieo_invariant_mid v1
-    else
-      bir_exp_false
-`;
-
-(* section is_even_2 *)
-val bir_ieo_sec_iseven_2_pre_def = Define `bir_ieo_sec_iseven_2_pre v1 =
-bir_ieo_invariant v1
-`;
-
-val bir_ieo_sec_iseven_2_post_def = Define `bir_ieo_sec_iseven_2_post v1 =
-bir_ieo_invariant_mid v1
-`;
-
-(* section is_odd_1 *)
-val bir_ieo_sec_isodd_1_pre_def = Define `bir_ieo_sec_isodd_1_pre v1 =
-bir_ieo_invariant_mid v1
-`;
-
-val bir_ieo_sec_isodd_1_post_def = Define `bir_ieo_sec_isodd_1_post v1 =
-\l. if l = BL_Address (Imm32 0x204w) then
+    else if l = BL_Address (Imm32 0x204w) then
       bir_ieo_ev_post_no v1
     else if l = BL_Address (Imm32 0x000w) then
       bir_ieo_invariant v1
@@ -127,15 +102,19 @@ val bir_ieo_sec_isodd_1_post_def = Define `bir_ieo_sec_isodd_1_post v1 =
       bir_exp_false
 `;
 
-(* section is_odd_2 *)
-val bir_ieo_sec_isodd_2_pre_def = Define `bir_ieo_sec_isodd_2_pre v1 =
-bir_ieo_invariant_mid v1
+
+(* section is_even exit post *)
+val bir_ieo_sec_iseven_exit_post_def = Define `bir_ieo_sec_iseven_exit_post v1 =
+\l. if l = BL_Address (Imm32 0x200w) then
+      bir_ieo_ev_post_yes v1
+    else if l = BL_Address (Imm32 0x204w) then
+      bir_ieo_ev_post_no v1
+    else if l = BL_Address (Imm32 0x000w) then
+      bir_exp_false
+    else
+      bir_exp_false
 `;
 
-val bir_ieo_sec_isodd_2_post_def = Define `bir_ieo_sec_isodd_2_post v1 =
-bir_ieo_invariant v1
-`;
-
 
 
 (* =============================================================== *)
@@ -144,46 +123,44 @@ bir_ieo_invariant v1
 
 
 
-val prefix = "bir_ieo_sec_iseven_1_";
+val prefix = "bir_ieo_sec_iseven_loop_";
 val first_block_label_tm = ``BL_Address (Imm32 0x000w)``;
-val ending_set =  ``{BL_Address (Imm32 0x200w); BL_Address (Imm32 0x100w);
-                     BL_Address (Imm32 0x204w); BL_Address (Imm32 0x000w)}``;
-val postcond_tm = ``bir_ieo_sec_iseven_1_post v1``;
+val ending_set =  ``{BL_Address (Imm32 0x200w); BL_Address (Imm32 0x000w); BL_Address (Imm32 0x204w)}``;
+val postcond_tm = ``bir_ieo_sec_iseven_post v1``;
 
-val defs = [bprog_is_even_odd_def, bir_ieo_sec_iseven_1_post_def,
-            bir_ieo_ev_post_yes_def, bir_ieo_invariant_mid_def,
+val defs = [bprog_is_even_odd_def, bir_ieo_sec_iseven_post_def,
+            bir_ieo_ev_post_no_def, bir_ieo_ev_post_yes_def, bir_ieo_invariant_def,
             bir_exp_false_def, BType_Bool_def];
 
-val (bir_ieo_sec_iseven_1_ht, bir_ieo_sec_iseven_1_wp_tm) =
+val (bir_ieo_sec_iseven_loop_ht, bir_ieo_sec_iseven_loop_wp_tm) =
   bir_obtain_ht prog_tm first_block_label_tm
                 ending_set ending_set_to_sml_list
                 postcond_tm postcond_exp_from_label
                 prefix defs;
 
-val bir_ieo_sec_iseven_1_wp_def =
-  Define `bir_ieo_sec_iseven_1_wp v1 = ^(bir_ieo_sec_iseven_1_wp_tm)`;
-val _ = save_thm (prefix ^ "ht", bir_ieo_sec_iseven_1_ht);
+val bir_ieo_sec_iseven_loop_wp_def =
+  Define `bir_ieo_sec_iseven_loop_wp v1 = ^(bir_ieo_sec_iseven_loop_wp_tm)`;
+val _ = save_thm (prefix ^ "ht", bir_ieo_sec_iseven_loop_ht);
 
 
 
-val prefix = "bir_ieo_sec_isodd_1_";
-val first_block_label_tm = ``BL_Address (Imm32 0x100w)``;
-val ending_set =  ``{BL_Address (Imm32 0x204w); BL_Address (Imm32 0x000w)}``;
-val postcond_tm = ``bir_ieo_sec_isodd_1_post v1``;
+val prefix = "bir_ieo_sec_iseven_exit_";
+val first_block_label_tm = ``BL_Address (Imm32 0x000w)``;
+val ending_set =  ``{BL_Address (Imm32 0x200w); BL_Address (Imm32 0x000w); BL_Address (Imm32 0x204w)}``;
+val postcond_tm = ``bir_ieo_sec_iseven_exit_post v1``;
 
-val defs = [bprog_is_even_odd_def, bir_ieo_sec_isodd_1_post_def,
-            bir_ieo_ev_post_no_def, bir_ieo_invariant_def,
+val defs = [bprog_is_even_odd_def, bir_ieo_sec_iseven_exit_post_def,
+            bir_ieo_ev_post_no_def, bir_ieo_ev_post_yes_def, bir_ieo_invariant_def,
             bir_exp_false_def, BType_Bool_def];
 
-val (bir_ieo_sec_isodd_1_ht, bir_ieo_sec_isodd_1_wp_tm) =
+val (bir_ieo_sec_iseven_exit_ht, bir_ieo_sec_iseven_exit_wp_tm) =
   bir_obtain_ht prog_tm first_block_label_tm
                 ending_set ending_set_to_sml_list
                 postcond_tm postcond_exp_from_label
                 prefix defs;
 
-val bir_ieo_sec_isodd_1_wp_def =
-  Define `bir_ieo_sec_isodd_1_wp v1 = ^(bir_ieo_sec_isodd_1_wp_tm)`;
-val _ = save_thm (prefix ^ "ht", bir_ieo_sec_isodd_1_ht);
-
+val bir_ieo_sec_iseven_exit_wp_def =
+  Define `bir_ieo_sec_iseven_exit_wp v1 = ^(bir_ieo_sec_iseven_exit_wp_tm)`;
+val _ = save_thm (prefix ^ "ht", bir_ieo_sec_iseven_exit_ht);
 
 val _ = export_theory();
