examples/tutorial/6-smt/tutorialExtra2_smtScript.sml
@@ -16,25 +16,44 @@ val _ = new_theory "tutorialExtra2_smt";
 
 
 
-val h_var_v1 = mk_var ("v1", Type `:word32`);
+val h_var_v1 = mk_var ("v1", Type `:word64`);
+val h_var_v  = mk_var ("v",  Type `:word64`);
 
-val get_contract_vars = (lhs o concl o (SPEC h_var_v1));
+val h_vars = [h_var_v1, h_var_v];
+
+fun get_contract_vars n = (lhs o concl o (SPECL (List.take(h_vars,n))));
 
 
-val contract_1_pre = get_contract_vars bir_ieo_sec_iseven_1_pre_def;
-val contract_1_wp  = get_contract_vars bir_ieo_sec_iseven_1_wp_def;
+val contract_1_pre = get_contract_vars 2 bir_ieo_sec_iseven_loop_pre_def;
+val contract_1_wp  = get_contract_vars 1 bir_ieo_sec_iseven_loop_wp_def;
 val contract_1_imp = bimp (contract_1_pre, contract_1_wp);
 
 val contract_1_imp_taut_thm = save_thm ("contract_1_imp_taut_thm",
   prove_exp_is_taut contract_1_imp);
 
 
-val contract_2_pre = get_contract_vars bir_ieo_sec_isodd_1_pre_def;
-val contract_2_wp  = get_contract_vars bir_ieo_sec_isodd_1_wp_def;
+val contract_2_pre = get_contract_vars 1 bir_ieo_sec_iseven_exit_pre_def;
+val contract_2_wp  = get_contract_vars 1 bir_ieo_sec_iseven_exit_wp_def;
 val contract_2_imp = bimp (contract_2_pre, contract_2_wp);
 
 val contract_2_imp_taut_thm = save_thm ("contract_2_imp_taut_thm",
   prove_exp_is_taut contract_2_imp);
+
+
+val contract_3_pre = ``bir_ieo_sec_iseven_exit_post v1 (BL_Address (Imm32 0w))``;
+val contract_3_wp  = get_contract_vars 1 bir_ieo_invariant_def;
+val contract_3_imp = bimp (contract_3_pre, contract_3_wp);
+
+val contract_3_imp_taut_thm = save_thm ("contract_3_imp_taut_thm",
+  prove_exp_is_taut contract_3_imp);
+
+
+val contract_4_pre = ``bir_ieo_ev_pre v1``;
+val contract_4_wp  = ``bir_ieo_invariant v1``;
+val contract_4_imp = bimp (contract_4_pre, contract_4_wp);
+
+val contract_4_imp_taut_thm = save_thm ("contract_4_imp_taut_thm",
+  prove_exp_is_taut contract_4_imp);
 
 
 val _ = export_theory();
